@prefix cc: <http://creativecommons.org/ns#>.
@prefix foaf: <http://xmlns.com/foaf/0.1/>.
@prefix owl: <http://www.w3.org/2002/07/owl#>.
@prefix rdf: <http://www.w3.org/1999/02/22-rdf-syntax-ns#>.
@prefix rdfs: <http://www.w3.org/2000/01/rdf-schema#>.
@prefix xsd: <http://www.w3.org/2001/XMLSchema#>.
@prefix sosa: <http://www.w3.org/ns/sosa/>.
@prefix mp: <http://www.example.com/TODO/>.

mp: a foaf:Document;
    foaf:primaryTopic mp:Ontology;
    cc:license <http://creativecommons.org/licenses/by/4.0/>.

mp:Ontology a owl:Ontology;
            rdfs:label "Matrix Profile Ontology"@en;
            rdfs:comment "Ontology for describing matrix profiles and matrix profile indexes"@en.

mp:matrixProfile a rdf:Property;
                 rdfs:label "Has matrix profile"@en;
                 rdfs:comment "A mp:matrixProfile is used to state that a series has a matrix profile"@en;
                 rdfs:range mp:MatrixProfile.

## MatrixProfile

mp:MatrixProfile a rdfs:Class;
                 rdfs:label "Matrix Profile"@en;
                 rdfs:comment "Defines a matrix profile"@en.

mp:windowSize a rdf:Property;
              rdfs:label "Window size"@en;
              rdfs:comment "Contains the window size that is used to calculate the matrix profile"@en;
              rdfs:domain mp:MatrixProfile;
              rdfs:range xsd:integer.

mp:belongsTo a rdf:Property;
             rdfs:label "Belongs to collection"@en;
             rdfs:comment "Contains the series that was used to calculate the matrix profile"@en;
             rdfs:domain mp:MatrixProfile.

## Result properties

mp:distance a rdf:Property;
         rdfs:label "Distance"@en;
         rdfs:comment "Distance from a feature of interest to it's nearest neighbor"@en;
         rdfs:range xsd:decimal.

mp:normalisedDistance a rdf:Property;
         rdfs:label "Normalised distance"@en;
         rdfs:comment "Normalised distance from a feature of interest to it's nearest neighbor"@en;
         rdfs:range xsd:decimal.

mp:nearestNeighbor a rdf:Property;
         rdfs:label "Nearest neighbor"@en;
         rdfs:comment "Contains the date of the nearest neighbor"@en;
         rdfs:range xsd:dateTime.
